\documentclass[11pt,a4paper]{article}
\usepackage{../ma319}
\semester{Fall}
\year{2019}
\subtitlenumber{1}
\author{刘逸灏 (515370910207)}

\begin{document}
\maketitle

\section{1.1/6}

对于$F(\xi)=F(x-at)$
$$\xi=x-at,\quad \frac{\partial \xi}{\partial t}=-a,\quad \frac{\partial \xi}{\partial x}=1,$$
$$\frac{\partial F}{\partial t}=\frac{\partial F}{\partial \xi}\cdot\frac{\partial \xi}{\partial t}=-aF'(\xi),$$
$$\frac{\partial^2 F}{\partial t^2}=\frac{\partial}{\partial t}[-aF'(\xi)]=\frac{\partial}{\partial \xi}[-aF'(\xi)]\cdot\frac{\partial \xi}{\partial t}=a^2F''(\xi),$$
$$\frac{\partial F}{\partial x}=\frac{\partial F}{\partial \xi}\cdot\frac{\partial \xi}{\partial x}=F'(\xi),$$
$$\frac{\partial^2 F}{\partial x^2}=\frac{\partial}{\partial x}[F'(\xi)]=\frac{\partial}{\partial \xi}[F'(\xi)]\cdot\frac{\partial \xi}{\partial x}=F''(\xi).$$

故$$\frac{\partial^2 F}{\partial t^2}-a^2\frac{\partial^2 F}{\partial x^2}=0.$$

对于$G(\xi)=G(x+at)$
$$\xi=x+at,\quad \frac{\partial \xi}{\partial t}=a,\quad \frac{\partial \xi}{\partial x}=1,$$
$$\frac{\partial G}{\partial t}=\frac{\partial G}{\partial \xi}\cdot\frac{\partial \xi}{\partial t}=aG'(\xi),$$
$$\frac{\partial^2 G}{\partial t^2}=\frac{\partial}{\partial t}[-aG'(\xi)]=\frac{\partial}{\partial \xi}[aG'(\xi)]\cdot\frac{\partial \xi}{\partial t}=a^2G''(\xi),$$
$$\frac{\partial G}{\partial x}=\frac{\partial G}{\partial \xi}\cdot\frac{\partial \xi}{\partial x}=G'(\xi),$$
$$\frac{\partial^2 G}{\partial x^2}=\frac{\partial}{\partial x}[G'(\xi)]=\frac{\partial}{\partial \xi}[G'(\xi)]\cdot\frac{\partial \xi}{\partial x}=G''(\xi).$$

故$$\frac{\partial^2 G}{\partial t^2}-a^2\frac{\partial^2 G}{\partial x^2}=0.$$

\section{1.1/7}

$$u(x,y,t)=(t^2-x^2-y^2)^{1/2},\quad t^2-x^2-y^2>0.$$

一阶偏导数为
$$\frac{\partial u}{\partial t}=\frac{1}{2}(t^2-x^2-y^2)^{-1/2}\cdot 2t=\frac{t}{u},$$
$$\frac{\partial u}{\partial x}=\frac{1}{2}(t^2-x^2-y^2)^{-1/2}\cdot -2x=-\frac{x}{u},$$
$$\frac{\partial u}{\partial y}=\frac{1}{2}(t^2-x^2-y^2)^{-1/2}\cdot -2y=-\frac{y}{u}.$$

二阶偏导数为
$$\frac{\partial^2 u}{\partial t^2}=\frac{\partial}{\partial t}\frac{t}{u}=\frac{\partial t}{\partial t}\cdot \frac{1}{u}+\frac{\partial}{\partial t}\frac{1}{u}\cdot t=\frac{1}{u}-\frac{3t^2}{u^3},$$
$$\frac{\partial^2 u}{\partial x^2}=-\frac{\partial}{\partial x}\frac{x}{u}=-\frac{\partial x}{\partial x}\cdot \frac{1}{u}-\frac{\partial}{\partial x}\frac{1}{u}\cdot t=-\frac{1}{u}-\frac{3x^2}{u^3},$$
$$\frac{\partial^2 u}{\partial y^2}=-\frac{\partial}{\partial y}\frac{y}{u}=-\frac{\partial y}{\partial y}\cdot \frac{1}{u}-\frac{\partial}{\partial y}\frac{1}{u}\cdot t=-\frac{1}{u}-\frac{3y^2}{u^3}.$$

故
$$\frac{\partial^2 u}{\partial t^2}-\frac{\partial^2 u}{\partial x^2}-\frac{\partial^2 u}{\partial y^2}=\frac{3}{u}+\frac{-3t^2+3x^2+3y^2}{u^3}=\frac{3}{u}+\frac{-3u^2}{u^3}=0,$$
$$\frac{\partial^2 u}{\partial t^2}=\frac{\partial^2 u}{\partial x^2}+\frac{\partial^2 u}{\partial y^2}.$$

\end{document}
